add resource maps and ectxt predicates

HeapLang/LanguageDefs.thy
@@ -25,20 +25,41 @@ fun lang_ctxt :: "langCtxt \<Rightarrow> expr \<Rightarrow> expr" where
 definition prim_step :: "expr \<Rightarrow> state \<Rightarrow> observation list \<Rightarrow> expr \<Rightarrow> state \<Rightarrow> expr list \<Rightarrow> bool" where
   "prim_step e1 \<sigma>1 \<kappa> e2 \<sigma>2 efs \<equiv> \<exists>K e1' e2'. ((e1=fill K e1') \<and> (e2=fill K e2') \<and> head_step e1' \<sigma>1 \<kappa> e2' \<sigma>2 efs)"
 
+lemma prim_step_simp: "head_step e1 \<sigma>1 \<kappa> e2 \<sigma>2 efs \<Longrightarrow> prim_step e1 \<sigma>1 \<kappa> e2 \<sigma>2 efs"
+  unfolding prim_step_def fill_def by (metis fold_simps(1))
+
 definition reducible :: "expr \<Rightarrow> state \<Rightarrow> bool" where
   "reducible e \<sigma> \<equiv> \<exists>\<kappa> e' \<sigma>' efs. prim_step e \<sigma> \<kappa> e' \<sigma>' efs"
+
+definition head_red :: "expr \<Rightarrow> state \<Rightarrow> bool" where
+  "head_red e \<sigma> \<equiv> \<exists>\<kappa> e' \<sigma>' efs. head_step e \<sigma> \<kappa> e' \<sigma>' efs"
 
 definition reducible_no_obs :: "expr \<Rightarrow> state \<Rightarrow> bool" where
   "reducible_no_obs e \<sigma> \<equiv> \<exists>e' \<sigma>' efs. prim_step e \<sigma> [] e' \<sigma>' efs"
 
+definition head_red_no_obs :: "expr \<Rightarrow> state \<Rightarrow> bool" where
+  "head_red_no_obs e \<sigma> \<equiv> \<exists>e' \<sigma>' efs. head_step e \<sigma> [] e' \<sigma>' efs"
+  
 definition irreducible :: "expr \<Rightarrow> state \<Rightarrow> bool" where
   "irreducible e \<sigma> \<equiv> \<forall>\<kappa> e' \<sigma>' efs. \<not>prim_step e \<sigma> \<kappa> e' \<sigma>' efs"
 
+definition head_irred :: "expr \<Rightarrow> state \<Rightarrow> bool" where
+  "head_irred e \<sigma> \<equiv> \<forall>\<kappa> e' \<sigma>' efs. \<not>head_step e \<sigma> \<kappa> e' \<sigma>' efs"
+  
 definition stuck :: "expr \<Rightarrow> state \<Rightarrow> bool" where
   "stuck e \<sigma> \<equiv> (to_val e = None) \<and> irreducible e \<sigma>"
 
+definition head_stuck :: "expr \<Rightarrow> state \<Rightarrow> bool" where
+  "head_stuck e \<sigma> \<equiv> (to_val e = None) \<and> head_irred e \<sigma>"
+  
 definition not_stuck :: "expr \<Rightarrow> state \<Rightarrow> bool" where
   "not_stuck e \<sigma> \<equiv> (\<exists>v. to_val e = Some v) \<or> reducible e \<sigma>"
+
+lemma head_red_no_obs_red: "head_red_no_obs e \<sigma> \<Longrightarrow> head_red e \<sigma>" 
+  by (auto simp: head_red_no_obs_def head_red_def)
+  
+lemma head_red_prim_step: "\<lbrakk>head_red e \<sigma>; prim_step e \<sigma> \<kappa> e' \<sigma>' efs\<rbrakk> \<Longrightarrow> head_step e \<sigma> \<kappa> e' \<sigma>' efs"
+sorry (* A rather strange proof in Coq that I don't want to replay right now. *)
 
 lemma irred_val: "irreducible (Val v) \<sigma>"
   unfolding irreducible_def prim_step_def
@@ -78,6 +99,55 @@ definition atomic :: "atomicity \<Rightarrow> expr \<Rightarrow> bool" where
   "atomic a e \<equiv> \<forall>\<sigma> e' \<kappa> \<sigma>' efs. prim_step e \<sigma> \<kappa> e' \<sigma>' efs \<longrightarrow> 
     (case a of WeaklyAtomic \<Rightarrow> irreducible e' \<sigma>' | StronglyAtomic \<Rightarrow> (\<exists>v. to_val e' = Some v))"
 
+definition head_atomic :: "atomicity \<Rightarrow> expr \<Rightarrow> bool" where
+  "head_atomic a e \<equiv> \<forall>\<sigma> e' \<kappa> \<sigma>' efs. head_step e \<sigma> \<kappa> e' \<sigma>' efs \<longrightarrow> 
+    (case a of WeaklyAtomic \<Rightarrow> irreducible e' \<sigma>' | StronglyAtomic \<Rightarrow> (\<exists>v. to_val e' = Some v))"
+    
+type_synonym lan_cfg = "expr list \<times> state"
+    
+definition step :: "lan_cfg \<Rightarrow> observation list \<Rightarrow> lan_cfg \<Rightarrow> bool" where
+  "step p1 \<kappa> p2 \<equiv> \<exists>t1 e1 t2 \<sigma>1 e2 efs \<sigma>2. p1 = (t1@e1#t2, \<sigma>1) \<and> p2 = (t1@e2#t2@efs, \<sigma>2) \<and>
+    prim_step e1 \<sigma>1 \<kappa> e2 \<sigma>2 efs"
+
+inductive nsteps :: "nat \<Rightarrow> lan_cfg \<Rightarrow> observation list \<Rightarrow> lan_cfg \<Rightarrow> bool" where
+  nsteps_refl: "nsteps 0 p [] p"
+| nsteps_l: "\<lbrakk>step p1 \<kappa> p2; nsteps n p2 \<kappa>s p3\<rbrakk> \<Longrightarrow> nsteps (Suc n) p1 (\<kappa>@\<kappa>s) p3"
+
+declare nsteps.intros[intro]
+inductive_cases nstepsE[elim]: "nsteps 0 p \<kappa> q"
+  "nsteps (Suc n) p \<kappa> q"
+
+definition pure_step :: "expr \<Rightarrow> expr \<Rightarrow> bool" where
+  "pure_step e1 e2 \<equiv> (\<forall>\<sigma>. reducible_no_obs e1 \<sigma>) \<and> 
+    (\<forall>\<sigma>1 \<kappa> e2' \<sigma>2 efs. prim_step e1 \<sigma>1 \<kappa> e2' \<sigma>2 efs \<longrightarrow> \<kappa> = [] \<and> \<sigma>2 = \<sigma>1 \<and> e2' = e2 \<and> efs = [])"
+
+definition pure_head_step :: "expr \<Rightarrow> expr \<Rightarrow> bool" where
+  "pure_head_step e1 e2 \<equiv> (\<forall>\<sigma>. head_red_no_obs e1 \<sigma>) \<and> 
+    (\<forall>\<sigma>1 \<kappa> e2' \<sigma>2 efs. head_step e1 \<sigma>1 \<kappa> e2' \<sigma>2 efs \<longrightarrow> \<kappa> = [] \<and> \<sigma>2 = \<sigma>1 \<and> e2' = e2 \<and> efs = [])"
+
+lemma pure_head_step_pure_step: "pure_head_step e1 e2 \<Longrightarrow> pure_step e1 e2"
+proof -
+  assume assm: "pure_head_step e1 e2"
+  then have no_obs: "head_red_no_obs e1 s" and 
+    head_step: "head_step e1 s1 k e2' s2 efs \<Longrightarrow> k = [] \<and> s2 = s1 \<and> e2' = e2 \<and> efs = []"
+    for s s1 k e2' s2 efs by (auto simp: pure_head_step_def)
+  from no_obs have no_obs': "\<forall>s. reducible_no_obs e1 s" 
+    apply (auto simp: reducible_no_obs_def head_red_no_obs_def )
+    using prim_step_simp by blast
+  from head_step[OF head_red_prim_step[OF head_red_no_obs_red[OF no_obs]]]
+  show ?thesis by (auto simp: pure_step_def no_obs')
+qed
+  
+abbreviation pure_exec :: "bool \<Rightarrow> nat \<Rightarrow> expr \<Rightarrow> expr \<Rightarrow> bool" where
+  "pure_exec P n e1 e2 \<equiv> P \<longrightarrow> rel_nsteps pure_step n e1 e2"
+
+lemma beta_red_no_obs: "head_red_no_obs (App (of_val (RecV f x e)) (of_val v)) \<sigma>"
+  by (auto simp: head_red_no_obs_def intro!: prim_step_simp)
+
+lemma pure_exec_beta: 
+  "pure_exec True 1 (App (Val (RecV f x e)) (Val v)) (subst' x v (subst' f (RecV f x e) e))" 
+  by (auto simp: pure_head_step_def beta_red_no_obs intro!: rel_one_step pure_head_step_pure_step)
+  
 text \<open>Atomicity proofs, but mostly axiomatized.\<close>
     
 lemma atomic_rec: "atomic a (Rec f x e)" 
